

Module-III

Interpolation

For any given pair of values (x_k, y_k) , $k = 0, 1, 2, 3, \dots, n$ with equal-spaced abscissas of a function $y = f(x)$, we defined the *forward difference operator* Δ as follows: The first forward difference is usually expressed as

$$\Delta y_i = y_{i+1} - y_i, \quad i = 0, 1, \dots, (n-1) \quad (22)$$

To be explicit, we write

$$\begin{aligned} \Delta y_0 &= y_1 - y_0 \\ \Delta y_1 &= y_2 - y_1 \\ &\vdots \\ \Delta y_{n-1} &= y_n - y_{n-1} \end{aligned}$$

These differences are called *first differences of the function y* and are denoted by the symbol Δy_i . Here, Δ is called *forward difference operator*.

Similarly, the difference of the first differences are called *second differences*, defined by

$$\Delta^2 y_0 = \Delta y_1 - \Delta y_0, \quad \Delta^2 y_1 = \Delta y_2 - \Delta y_1$$

Thus, in general

$$\Delta^2 y_i = \Delta y_{i+1} - \Delta y_i$$

Here Δ^2 is called the *second difference operator*. Thus, continuing, we can define, r^{th} difference of y , as

$$\Delta^r y_t = \Delta^{r-1} y_{t+1} - \Delta^{r-1} y_t \quad (23)$$

x	y	Δy	$\Delta^2 y$	$\Delta^3 y$	$\Delta^4 y$	$\Delta^5 y$
x_0	y_0					
x_1	y_1	Δy_0				
$(= x_0 + h)$			$\Delta^2 y_0$			
x_2	y_2	Δy_1	$\Delta^2 y_1$	$\Delta^3 y_0$		
$(= x_0 + 2h)$				$\Delta^3 y_1$	$\Delta^4 y_0$	
x_3	y_3	Δy_2	$\Delta^2 y_2$	$\Delta^3 y_2$	$\Delta^4 y_1$	$\Delta^5 y_0$
$(= x_0 + 3h)$						
x_4	y_4	Δy_3	$\Delta^2 y_3$			
$(= x_0 + 4h)$						
x_5	y_5	Δy_4				
$(= x_0 + 5h)$						

Figure 5: Forward difference table

It can be noted that the subscription remains constant along each diagonal of the table. The first term in the table, that is y_0 is called the *leading term*, while the differences $\Delta y_0, \Delta^2 y_0, \Delta^3 y_0, \dots$ are called leading differences.

Example 3.2.1

Express $\Delta^2 y_0$ and $\Delta^3 y_0$ in terms of the values of the function y .

Noting that each higher order difference is defined in terms of the lower order difference, we have

$$\Delta^2 y_0 = \Delta y_1 - \Delta y_0 = (y_2 - y_1) - (y_1 - y_0) = y_2 - 2y_1 + y_0$$

and

$$\begin{aligned}\Delta^3 y_0 &= \Delta^2 y_1 - \Delta^2 y_0 = (\Delta y_2 - \Delta y_1) - (\Delta y_1 - \Delta y_0) \\ &= (y_3 - y_2) - (y_2 - y_1) - (y_2 - y_1) + (y_1 - y_0) \\ &= y_3 - 3y_2 + 3y_1 - y_0.\end{aligned}$$

$$\Delta^4 y_0 = y_4 - 4y_3 + 6y_2 - 4y_1 + y_0.$$

Hence, we observed that the coefficients of the values of y , in the expansion of $\Delta^2 y_0$, $\Delta^3 y_0$ are binomial coefficients. Thus, in general, we arrive at the following result.

$$\Delta^n y_0 = y_n - {}^n C_1 y_{n-1} + {}^n C_2 y_{n-2} - {}^n C_3 y_{n-3} + \cdots + (-1)^n y_0$$



Example 3.2.2

Prove that


$$\textcircled{1} \quad \Delta(f(x) + g(x)) = \Delta f(x) + \Delta g(x).$$

$$\textcircled{2} \quad \Delta cy(n) = c\Delta y(n)$$

$$\textcircled{3} \quad \Delta(cx_n + cy_n) = c\Delta x_n + c\Delta y_n$$

$$\begin{aligned}\Delta(f(x) + g(x)) &= (f(x+1) + g(x+1)) - (f(x) + g(x)) \\ &= (f(x+1) - f(x)) + (g(x+1) - g(x)) \\ &= \Delta f(x) + \Delta g(x).\end{aligned}\tag{25}$$

$$\begin{aligned}\Delta cy(n) &= cy(n+1) - cy(n) \\ &= c(y(n+1) - y(n)) = c\Delta y(n)\end{aligned}\tag{26}$$

From Eq.25 and Eq.26, it is proved that $\Delta(cx_n + cy_n) = c\Delta x_n + c\Delta y_n$.  **VIT**
BHOPAL
www.vitbhopal.ac.in

Δ is a linear operator.

Example 3.3.1

Construct a forward difference table for the following values of x and y :

x	0.1	0.3	0.5	0.7	0.9	1.1	1.3
y	0.003	0.067	0.148	0.248	0.370	0.518	0.697

x	y	Δy	$\Delta^2 y$	$\Delta^3 y$	$\Delta^4 y$	$\Delta^5 y$	$\Delta^6 y$
0.1	0.003						
		0.064					
0.3	0.067		0.017				
		0.081		0.002			
0.5	0.148		0.019		0.001		
		0.1		0.003		0	
0.7	0.248		0.022		0.001		0
		0.122		0.004		0	
0.9	0.37		0.026		0.001		
		0.148		0.005			
1.1	0.518		0.031				
		0.179					
1.3	0.697						

Practice problem

- ① Construct a forward difference table for the following set of values:

x_i	0	2	4	6	8	10	12	14
y_i	625	81	1	1	81	625	2401	65611

- ② Construct a forward (diagonal) difference table for the following set of values:

x_i	1	2	3	4	5
y_i	4	13	34	73	136

Example 3.4.1

Using Newton's forward formula. find the value of $\sin 52^\circ$ from the following:

θ°	45°	50°	55°	60°
$\sin \theta$	0.7071	0.7660	0.8192	0.8660

Solution:

θ°	$\sin \theta$	Δ	Δ^2	Δ^3
45°	0.7071			
		0.0589		
50°	0.7660		-0.0057	
		0.0532		-0.0007
55°	0.8192		-0.0064	
		0.0468		
60°	0.8660			

Applying Newton's forward difference interpolation formula.

$$y_n(x) = y_0 + p\Delta y_0 + \frac{p(p-1)}{2!}\Delta^2 y_0 + \frac{p(p-1)(p-2)}{3!}\Delta^3 y_0 + \dots$$

Here $y_n(x) = \sin 52^\circ$

$$y_0 = 0.7071, \Delta y_0 = 0.0589, \Delta^2 y_0 = -0.0057, \Delta^3 y_0 = -0.0007$$

$$h = x_1 - x_0 = 50 - 45 = 5$$

$$p = \frac{x - x_0}{h} = \frac{52 - 45}{5} = \frac{7}{5} = 1.4$$

$$\sin 52^\circ = 0.7071 + (1.4)(0.0589) + \frac{1.4(0.4)}{2}(-0.0057)$$

$$+ \frac{1.4(0.4)(-0.6)}{6}(-0.0007)$$

$$= 0.7071 + 0.08246 - 0.0016 + 0.00004$$

$$\sin 52^\circ = 0.7880$$

Example 3.4.2

Using Newton's forward formula, find the value of $f(218)$ if,

x	100	150	200	250	300	350	400
$f(x)$	10.63	13.03	15.04	16.81	18.42	19.90	21.27

x	$f(x)$	Δ	Δ^2	Δ^3	Δ^4	Δ^5	Δ^6
100	10.63						
		2.4					
150	13.03		-0.39				
		2.01		0.15			
200	15.04		-0.24		-0.07		
		1.77		0.08		0.02	
250	16.81		-0.16		-0.05		0.02
		1.61		0.03		0.04	
300	18.42		-0.13		-0.01		
		1.48		0.02			
350	19.90		-0.11				
		1.37					
400	21.27						

$$\begin{aligned}
 y_n(x) = & y_0 \\
 & + p\Delta y_0 \\
 & + \frac{p(p-1)}{2!}\Delta^2 y_0 \\
 & + \frac{p(p-1)(p-2)}{3!}\Delta^3 y_0 \\
 & + \frac{p(p-1)(p-2)(p-3)}{4!}\Delta^4 y_0 \\
 & + \frac{p(p-1)(p-2)(p-3)(p-4)}{5!}\Delta^5 y_0 \\
 & + \frac{p(p-1)(p-2)(p-3)(p-4)(p-5)}{6!}\Delta^6 y_0
 \end{aligned}$$

Here

$$h = x_1 - x_0 = 150 - 100 = 50$$

$$y_n(x) = f(218), p = \frac{x - x_0}{h} = \frac{218 - 100}{50} = 2.36$$

$$\begin{aligned}
f(218) &= 10.63 + (2.36)(2.4) \\
&+ \frac{(2.36)(1.36)}{2}(-0.39) \\
&+ \frac{(2.36)(1.36)(0.36)}{6}(-0.39) \\
&+ \frac{(2.36)(1.36)(0.36)(-0.64)}{24}(0.15) \\
&+ \frac{(2.36)(1.36)(0.36)(-0.64)(-1.64)}{120}(-0.07) \\
&+ \frac{(2.36)(1.36)(0.36)(-0.64)(-1.64)(-2.64)}{720}(0.02) \\
&= 10.63 + 5.664 - 0.6259 + 0.0289 + 0.0022 + 0 + 0 \\
f(218) &= 15.6993
\end{aligned}$$

Example 3.4.3

The table gives the distance in nautical miles of the visible horizon for the given heights in feet above the earth's surface:

$x = \text{height}$	100	150	200	250	300	350	400
$y = \text{distance}$	10.63	13.03	15.04	16.81	18.42	19.90	21.27

Find the values of y when $x = 160\text{ft}..$

x	$f(x)$	Δ	Δ^2	Δ^3	Δ^4	Δ^5	Δ^6
100	10.63						
		2.4					
150	13.03		-0.39				
		2.01		0.15			
200	15.04		-0.24		-0.07		
		1.77		0.08		0.02	
250	16.81		-0.16		-0.05		0.02
		1.61		0.03		0.04	
300	18.42		-0.13		-0.01		
		1.48		0.02			
350	19.90		-0.11				
		1.37					
400	21.27						

The value of x at $f(x) : x = 160$.

$$h = x_1 - x_0 = 150 - 100 = 50$$

$$p = \frac{x - x_0}{h} = \frac{160 - 100}{50} = 1.2$$

$$\begin{aligned} y_n(x) = & y_0 + p\Delta y_0 + \frac{p(p-1)}{2!}\Delta^2 y_0 + \frac{p(p-1)(p-2)}{3!}\Delta^3 y_0 \\ & + \frac{p(p-1)(p-2)(p-3)}{4!}\Delta^4 y_0 \\ & + \frac{p(p-1)(p-2)(p-3)(p-4)}{5!}\Delta^5 y_0 \\ & + \frac{p(p-1)(p-2)(p-3)(p-4)(p-5)}{6!}\Delta^6 y_0 \end{aligned}$$

$$y(160) = 10.63 + 2.88 - 0.0468 - 0.0048 - 0.001 + 0 + 0$$

$$y(160) = 13.4573$$

Example 3.4.4

Find the polynomial which satisfies the following table of values.

x	1	2	3	4	5	6	7	8
y	2	9	22	41	66	97	134	177

x	y	Δ	Δ^2	Δ^3	Δ^4	Δ^5	Δ^6	Δ^7
1	2							
		7						
2	9		6					
		13		0				
3	22		6		0			
		19		0		0		
4	41		6		0		0	
		25		0		0		0
5	66		6		0		0	
		31		0		0		
6	97		6		0			
		37		0				
7	134		6					
		43						
8	177							

x	$f(x) = ax^2 + bx + c$	Δ	Δ^2	Δ^3	Δ^4	Δ^5	Δ^6	Δ^7
1	$a+b+c$							
		$3a+b$						
2	$4a+2b+c$		$2a$					
		$5a+b$		0				
3	$9a+3b+c$		$2a$		0			
		$7a+b$		0		0		
4	$16a+4b+c$		$2a$		0		0	
		$9a+b$		0		0		0
5	$25a+5b+c$		$2a$		0		0	
		$11a+b$		0		0		
6	$36a+6b+c$		$2a$		0			
		$13a+b$		0				
7	$49a+7b+c$		$2a$					
		$15a+b$						
8	$64a+8b+c$							

Now, comparing Δ^2 column of both tables, then we

$$2a = 6$$

$$a = 3$$

Comparing Δ column of both tables, then we

$$3a + b = 7$$

$$9 + b = 7$$

$$b = -2$$

Comparing $f(x)$ column of both tables, then we

$$a + b + c = 2$$

$$3 - 2 + c = 2$$

$$c = 1$$

So, the desired polynomial is

$$f(x) = 3x^2 - 2x + 1$$

Example 3.4.5

Find the polynomial that satisfies the following table of values

x	-3	-2	-1	0	1	2	3
y	0	-4	0	6	8	0	-24

x	y	Δ	Δ^2	Δ^3	Δ^4	Δ^5	Δ^6
-3	0						
		-4					
-2	-4		8				
		4		-6			
-1	0		2		0		
		6		-6		0	
0	6		-4		0		0
		2		-6		0	
1	8		-10		0		
		-8		-6			
2	0		-24				
		-24					
3	-24						

$$a = -1; b = -2; c = 5; d = 6$$

$$f(x) = -x^3 - 2x^2 = 5x + 6$$

Example 3.4.6

Determine the value of constant finite differences

① $f(x) = 3x^2 - x + 2$

② $f(x) = -2x^3 + 3x^2 + x - 1$

Formula to find constant finite differences

Constant finite differences = (Degree of the polynomial)! \times leading coefficient

1. Here,

Leading coefficient = 3 and Degree of the polynomial = 2

Constant finite differences = $2! \times 3$

2. Here,

Leading coefficient = -2 and Degree of the polynomial = 3

Constant finite differences = $3! \times -2 = -12$

Definition 3.5.1 (Backward Differences)

The differences $y_1 - y_0, y_2 - y_1, \dots, y_n - y_{n-1}$ when denoted by $\nabla y_1, \nabla y_2, \dots, \nabla y_n$, respectively, are called first backward difference. Thus, the first backward differences are $\nabla y_r = y_r - y_{r-1}$. This formula is useful when the value of $f(x)$ is required near the end of the table. h is called the interval of difference and $u = \frac{x-x_n}{h}$, Here x_n is last term.

x	y	∇y	$\nabla^2 y$	$\nabla^3 y$	$\nabla^4 y$	$\nabla^5 y$
x_0	y_0					
x_1	y_1	∇y_1				
$(= x_0 + h)$			$\nabla^2 y_2$			
x_2	y_2	∇y_2	$\nabla^2 y_3$	$\nabla^3 y_3$		
$(= x_0 + 2h)$		∇y_3		$\nabla^3 y_4$	$\nabla^4 y_4$	
x_3	y_3	∇y_4	$\nabla^2 y_4$	$\nabla^3 y_5$	$\nabla^4 y_5$	$\nabla^5 y_5$
$(= x_0 + 3h)$			$\nabla^2 y_5$			
x_4	y_4	∇y_5				
$(= x_0 + 4h)$						
x_5	y_5					
$(= x_0 + 5h)$						

Figure 6: Backward difference table

Example 3.5.2

Given $\sin 45^\circ = 0.7071$, $\sin 50^\circ = 0.7660$, $\sin 55^\circ = 0.8192$, $\sin 60^\circ = 0.8660$. Find $\sin 57^\circ$ using on appropriate interpolation formula.

We can form a table of values as follows

x	45°	50°	55°	60°
y	0.7071	0.7660	0.8192	0.8660

Since $\sin 57^\circ$ is closer x_n value, we can choose Newton's backward interpolation formula.

x	y	∇	∇^2	∇^3
45°	0.7071			
		0.0589		
50°	0.7660		-0.0057	
		0.0532		-0.0007
55°	0.8192		-0.0064	
		0.0468		
60°	0.8660			

Here,

$$r = \frac{x - x_n}{h} = \frac{57 - 60}{5} = -0.6$$

We have newton's backward interpolation formula

$$y_r = y_n + r\nabla y_n + \frac{(r)(r+1)}{2!}\nabla^2 y_n + \frac{(r)(r+1)(r+2)}{3!}\nabla^3 y_n + \dots$$

$$\begin{aligned} y_{57} &= 0.8660 + (-0.6)(0.0468) + \frac{(-0.6)(-0.6+1)}{2!}(-0.0064) \\ &\quad + \frac{(-0.6)(0.6+1)(0.6+2)}{3!}(-0.0007) \end{aligned}$$

$$\sin(57) = 0.8387$$

Example 3.5.3

Find the value of $f(17)$ from following table of values

x	0	5	10	15	20
$f(x)$	1.0	1.6	3.8	8.2	15.4

x	$f(x)$	∇y_n	$\nabla^2 y_n$	$\nabla^3 y_n$	$\nabla^4 y_n$
0	1.0				
		6			
5	1.6		1.6		
		2.2		0.6	
10	3.8		2.2		0
		4.4		0.6	
15	8.2		4.4		
		7.2			
20	15.4				

Here,

$$r = \frac{17 - 20}{5} = -0.6$$

We have newton's backward interpolation formula

$$y_r = y_n + r\nabla y_n + \frac{(r)(r+1)}{2!}\nabla^2 y_n \\ + \frac{(r)(r+1)(r+2)}{3!}\nabla^3 y_n + \dots$$

$$y_{57} = 15.4 + (-0.6)(7.2) + \frac{(-0.6)(-0.6+1)}{2!}(4.4) \\ + \frac{(-0.6)(-0.6+1)(-0.6+2)}{3!}(0.6) \\ + \frac{(-0.6)(-0.6+1)(-0.6+2)(0.6+3)}{4!}(0)$$

$$f(17) = 10.5184$$

Problem 3.5.4

Given the following data estimate $f(4.12)$ using Newton-Gregory backward difference interpolation polynomial:

x	0	1	2	3	4	5
$f(x)$	1	2	4	8	16	32

Lagrange Interpolation Formula

Suppose we have one point $(1, 3)$. How can we find a polynomial that could represent it?

$$P(x) = 3$$

$$P(x) = 3x$$

$$P(1) = 3$$

Suppose we have sequence of points: $(1, 3), (2, 4)$. How can we find a polynomial that could represent it?

$$P(x) = \frac{(x-2)}{(1-2)} \times 3 + \frac{(x-1)}{(2-1)} \times 4$$

$$P(x) = x + 2$$

$$P(1) = 3$$

$$P(2) = 4$$

Suppose we have sequence of points: $(1, 3), (2, 4), (7, 11)$. How can we find a polynomial that could represent it?

$$P(x) = \frac{(x-2)(x-7)}{(1-2)(1-7)} \times 3 + \frac{(x-1)(x-7)}{(2-1)(2-7)} \times 4 + \frac{(x-1)(x-2)}{(7-1)(7-2)} \times 11$$

$$P(1) = 3$$

$$P(2) = 4$$

$$P(7) = 11$$

In a general form it looks like this:

$$P(x) = \frac{(x-x_2)(x-x_3)}{(x_1-x_2)(x_1-x_3)}y_1 + \frac{(x-x_1)(x-x_3)}{(x_2-x_1)(x_2-x_3)}y_2 + \frac{(x-x_1)(x-x_2)}{(x_3-x_1)(x_3-x_2)}y_3$$

$$P(x) = \sum_1^3 P_i(x)y_i$$

Definition 3.6.1 (Formula to find the function value)

$$y = \frac{(x - x_1)(x - x_2) \cdots (x - x_n)}{(x_0 - x_1)(x_0 - x_2) \cdots (x_0 - x_n)} y_0 + \frac{(x - x_0)(x - x_2) \cdots (x - x_n)}{(x_1 - x_0)(x_1 - x_2) \cdots (x_1 - x_n)} y_1$$
$$+ \cdots + \frac{(x - x_1)(x - x_1) \cdots (x - x_{n-1})(x_n - x_0)}{(x_0 - x_1) \cdots (x_n - x_{n-1})} y_n$$
$$y = V_0(x_n) y_0 + V_1(x_n) y_1 + V_2(x_n) y_2 + V_3(x_n) y_3 + \cdots + V_n(x_n) y_n$$

Definition 3.6.2 (Find the Polynomial of the given data)

$$P(x) = \sum_{j=0}^n y_j \left(\prod_{i=0, i \neq j}^n \frac{x - x_i}{x_j - x_i} V_i(x) y_i \right)$$

Example 3.6.3

Using the Lagrange interpolation formula, find the value of y at $x = 0$ given some set of values $(-2, 5)$, $(1, 7)$, $(3, 11)$, $(7, 34)$?

Solution:

$$\begin{aligned} y(x) = & \frac{(x - x_1)(x - x_2)(x - x_3)}{(x_0 - x_1)(x_0 - x_2)(x_0 - x_3)}y_0 + \frac{(x - x_0)(x - x_2)(x - x_3)}{(x_1 - x_0)(x_1 - x_2)(x_1 - x_3)}y_1 \\ & + \frac{(x - x_0)(x - x_1)(x - x_3)}{(x_2 - x_0)(x_2 - x_1)(x_2 - x_3)}y_2 + \frac{(x - x_0)(x - x_1)(x - x_2)}{(x_3 - x_0)(x_3 - x_1)(x_3 - x_2)}y_3 \end{aligned}$$

Given the known values are, $x = 0; x_0 = -2; x_1 = 1; x_2 = 3; x_3 = 7; y_0 = 5;$
 $y_1 = 7; y_2 = 11; y_3 = 34.$

$$\begin{aligned}
 y &= \frac{(0-1)(0-3)(0-7)}{(-2-1)(-2-3)(-2-7)} \times 5 + \frac{(0-(-2))(0-3)(0-7)}{(1-(-2))(1-3)(1-7)} \times 7 \\
 &+ \frac{(0-(-2))(0-1)(0-7)}{(3-(-2))(3-1)(3-7)} \times 11 + \frac{(0-(-2))(0-1)(0-3)}{(7-(-2))(7-1)(7-3)} \times 34 \\
 y &= \frac{21}{27} + \frac{49}{6} + \frac{-77}{20} + \frac{51}{54} \\
 y &= \frac{1087}{180}
 \end{aligned}$$

Example 3.6.4

Consider the following table of functional values, find $f(0.06)$ using Lagrange interpolation, where function generated with $f(x) = \log(x)$.

i	x_i	f_i
0	0.40	-0.916291
1	0.50	-0.693147
2	0.70	-0.356675
3	0.80	-0.223144

$$\begin{aligned} f(x) = & \frac{(x - x_1)(x - x_2)(x - x_3)}{(x_0 - x_1)(x_0 - x_2)(x_0 - x_3)}f_0 + \frac{(x - x_0)(x - x_2)(x - x_3)}{(x_1 - x_0)(x_1 - x_2)(x_1 - x_3)}f_1 \\ & + \frac{(x - x_0)(x - x_1)(x - x_3)}{(x_2 - x_0)(x_2 - x_1)(x_2 - x_3)}f_2 + \frac{(x - x_0)(x - x_1)(x - x_2)}{(x_3 - x_0)(x_3 - x_1)(x_3 - x_2)}f_3 \end{aligned}$$

$$\begin{aligned}
 y(0.06) &= \frac{(0.06 - 0.50)(0.06 - 0.70)(0.06 - 0.80)}{(0.40 - 0.50)(0.40 - 0.70)(0.40 - 0.80)} \times -0.9163 \\
 &+ \frac{(0.06 - 0.40)(0.06 - 0.70)(0.06 - 0.80)}{(0.50 - 0.40)(0.50 - 0.70)(0.50 - 0.80)} \times -0.6931 \\
 &+ \frac{(0.06 - 0.40)(0.06 - 0.50)(0.06 - 0.80)}{(0.70 - 0.40)(0.70 - 0.50)(0.70 - 0.80)} \times -0.3567 \\
 &+ \frac{(0.06 - 0.40)(0.06 - 0.50)(0.06 - 0.70)}{(0.80 - 0.40)(0.80 - 0.50)(0.80 - 0.70)} \times -0.2231
 \end{aligned}$$

$$\begin{aligned}
 y(0.06) &= \frac{(-0.44)(-0.64)(-0.74)}{(-0.10)(-0.30)(-0.40)}(-0.9163) + \frac{(-0.34)(-0.64)(-0.74)}{(0.10)(-0.20)(-0.30)}(-0.6931) \\
 &+ \frac{(-0.34)(-0.44)(-0.74)}{(0.30)(0.20)(-0.10)}(-0.3567) + \frac{(-0.34)(-0.44)(-0.64)}{(0.40)(0.30)(0.10)}(-0.2231)
 \end{aligned}$$

$$\begin{aligned}
 y(0.06) &= \frac{-0.2084}{-0.012} \times -0.9163 + \frac{-0.161}{0.006} \times -0.6931 \\
 &\quad + \frac{-0.1107}{-0.006} \times -0.3567 + \frac{-0.0957}{0.012} \times -0.2231 \\
 y(0.06) &= -2.11
 \end{aligned}$$

Solution of the polynomial at point 0.06 is $y(0.06) = -2.11$

Problem

Using Lagrange interpolation to find a polynomial P of degree < 4 satisfying

$$P_1(1) = 1, P_2(2) = 4, P_3(3) = 1, P_4(4) = 5,$$

what are the polynomials $P_1(x), P_2(x), P_3(x), P_4(x), P(x)$?

Solution:

Let $f(x_0) = (x_0 - x_1)(x_0 - x_2)(x_0 - x_3)$. Then $f(1) = (-1)(-2)(-3) = -6$.
So,

$$P_1(x) = (x - x_1)(x - x_2)(x - x_3) = \frac{-1}{6}(x - 2)(x - 3)(x - 4).$$

Let $f(x_1) = (x_1 - x_0)(x_1 - x_2)(x_1 - x_3)$. Then $f(2) = (1)(-1)(-2) = 2$. So,

$$P_2(x) = (x - x_0)(x - x_2)(x - x_3) = \frac{1}{2}(x - 1)(x - 3)(x - 4).$$

Let $f(x_2) = (x_2 - x_0)(x_2 - x_1)(x_2 - x_3)$. Then $f(3) = (2)(1)(-1) = -2$. So,

$$P_3(x) = (x - x_0)(x - x_1)(x - x_3) = \frac{-1}{2}(x - 1)(x - 2)(x - 4).$$

Let $f(x_3) = (x_3 - x_0)(x_3 - x_1)(x_3 - x_2)$. Then $f(4) = (3)(2)(1) = 6$. So,

$$P_4(x) = (x - x_0)(x - x_1)(x - x_2) = \frac{1}{6}(x - 1)(x - 2)(x - 3).$$

Hence,

$$\begin{aligned} P(x) &= P_1(x)y_0 + P_2(x)y_1 + P_3(x)y_2 + P_4(x)y_3 \\ &= \left(\left(-\frac{1}{6} \right) (x - 2)(x - 3)(x - 4) \right) 1 + \left(\left(\frac{1}{2} \right) (x - 1)(x - 3)(x - 4) \right) 4 \\ &\quad + \left(\left(-\frac{1}{2} \right) (x - 1)(x - 2)(x - 4) \right) 1 + \left(\left(\frac{1}{6} \right) (x - 1)(x - 2)(x - 3) \right) 5. \end{aligned}$$

Simplifying gives $P(x) = \frac{13}{6}x^3 - 16x^2 + \frac{215}{6}x - 21$.

Problem 3.6.5

Given the following data:

$x_0 = 3$	$f_0 = 1$
$x_1 = 4$	$f_1 = 2$
$x_2 = 5$	$f_2 = 4$

Find the quadratic interpolating function $g(x)$.

Lagrange basis functions are

$$V_0(x) = \frac{(x-4)(x-5)}{(3-4)(3-5)}$$

$$V_1(x) = \frac{(x-3)(x-5)}{(4-3)(4-5)}$$

$$V_2(x) = \frac{(x-3)(x-4)}{(5-3)(5-4)}$$

Interpolating function $g(x)$ is: $g(x) = 1.0V_0(x) + 2.0V_1(x) + 4.0V_2(x)$.

Newton's divided difference interpolation

x_i	f_i	$f[x_i, x_j]$	$f[x_i, x_j, x_k]$	$f[x_i, x_j, x_k, x_l]$
x_0	f_0			
		$f[x_0, x_1]$ $= \frac{f_1 - f_0}{x_1 - x_0}$		
x_1	f_1		$f[x_0, x_1, x_2]$ $= \frac{f[x_1, x_2] - f[x_0, x_1]}{x_2 - x_0}$	
		$f[x_1, x_2]$ $= \frac{f_2 - f_1}{x_2 - x_1}$		$f[x_0, x_1, x_2, x_3]$ $= \frac{f[x_1, x_2, x_3] - f[x_0, x_1, x_2]}{x_3 - x_0}$
x_2	f_2		$f[x_1, x_2, x_3]$ $= \frac{f[x_2, x_3] - f[x_1, x_2]}{x_3 - x_1}$	
		$f[x_2, x_3]$ $= \frac{f_3 - f_2}{x_3 - x_2}$		
x_3	f_3			

$$f(x) = f[x_0] + (x - x_0)f[x_0, x_1] + (x - x_0)(x - x_1)f[x_0, x_1, x_2] + (x - x_0)(x - x_1)(x - x_2)f[x_0, x_1, x_2, x_3]$$

Example 3.7.1

Find solution of $f(x)$ when $x = 151.23855$ using Newton's divided difference interpolation formula for the following data.

x	300	304	305
f(x)	2.4771	2.4829	2.4843

x	y	1st order	2nd order
300	2.4771		
		$\frac{2.4829 - 2.4771}{304 - 300}$ $= 0.0014$	
304	2.4829		$\frac{0.0014 - 0.0014}{305 - 300}$ $= 0$
		$\frac{2.4843 - 2.4829}{305 - 304}$ $= 0.0014$	
305	2.4843		

Newton's divided difference interpolation

The value of x at you want to find the $f(x) : x = 151.23855$.

Newton's divided difference interpolation formula is

$$f(x) = y_0 + (x - x_0)f[x_0, x_1] + (x - x_0)(x - x_1)f[x_0, x_1, x_2]$$

$$\begin{aligned}y(151.23855) &= 2.4771 + (151.23855 - 300) \times 0.0014 \\&\quad + (151.23855 - 300)(151.23855 - 304) \times 0\end{aligned}$$

$$\begin{aligned}y(151.23855) &= 2.4771 + (-148.7614) \times 0.0014 \\&\quad + (-148.7614)(-152.7614) \times 0\end{aligned}$$

$$y(151.23855) = 2.4771 - 0.2083 + 0$$

$$y(151.23855) = 2.2688$$

Solution of divided difference interpolation method $y(151.23855) = 2.2688$

Problem 3.7.2

The upward velocity of a rocket is given as a function of time in the following Table

$t(s)$	0	10	15	20	22.5	30
$v(t)(m/s)$	0	227.04	362.78	517.35	602.97	901.67

- Ⓐ Determine the value of the velocity at $t = 16$ seconds using Newton's divided difference polynomial method.
- Ⓑ Using the third order polynomial interpolant for velocity, find the distance covered by the rocket from $t = 11s$ to $t = 16s$.
- Ⓒ Using the third order polynomial interpolant for velocity, find the acceleration of the rocket at $t = 16s$.

(a)

x	y	1 st order	2 nd order	3 rd order	4 th order	5 th order
$x_0 = 0$	$y_0 = 0$					
		22.704				
$x_1 = 10$	227.04		0.2963			
		27.148		0.004		
$x_2 = 15$	362.78		0.3766		0.0001	
		30.914		0.0054		0
$x_3 = 20$	517.35		0.4445		0.0001	
		34.248		0.0076		
$x_4 = 22.5$	602.97		0.5579			
		39.8267				
$x_5 = 30$	901.67					

The value of x at you want to find the $f(x) : x = 16$ Newton's divided difference interpolation formula is

$$\begin{aligned} f(x) &= y_0 + (x - x_0)f[x_0, x_1] \\ &+ (x - x_0)(x - x_1)f[x_0, x_1, x_2] \\ &+ (x - x_0)(x - x_1)(x - x_2)f[x_0, x_1, x_2, x_3] \\ &+ (x - x_0)(x - x_1)(x - x_2)(x - x_3)f[x_0, x_1, x_2, x_3, x_4] \\ &+ (x - x_0)(x - x_1)(x - x_2)(x - x_3)(x - x_4)f[x_0, x_1, x_2, x_3, x_4, x_5] \end{aligned}$$

$$y(16) = 0 + (16 - 0) \times 22.704 + (16 - 0)(16 - 10) \times 0.2963$$

$$+ (16 - 0)(16 - 10)(16 - 15) \times 0.004$$

$$+ (16 - 0)(16 - 10)(16 - 15)(16 - 20) \times 0.0001$$

$$+ (16 - 0)(16 - 10)(16 - 15)(16 - 20)(16 - 22.5) \times 0$$

$$y(16) = 0 + (16) \times 22.704 + (16)(6) \times 0.2963 + (16)(6)(1) \times 0.004$$

$$+ (16)(6)(1)(-4) \times 0.0001 + (16)(6)(1)(-4)(-6.5) \times 0$$

$$y(16) = 0 + 363.264 + 28.4448 + 0.384 - 0.0384 + 0$$

$$y(16) = 392.0544$$

Solution of divided difference interpolation method $y(16) = 392.0544$

(b). The distance covered by the rocket between $t = 11s$ and $t = 16s$ can be calculated from the interpolating polynomial

$$\begin{aligned}v(t) &= y_1 + f[x_1, x_2](t - x_1) + f[x_1, x_2, x_3](t - x_1)(t - x_2) \\&\quad + f[x_1, x_2, x_3, x_4](t - x_1)(t - x_2)(t - x_3) \\v(t) &= 227.04 + 27.148(t - 10) + 0.37660(t - 10)(t - 15) \\&\quad + 0.005434 \times (t - 10)(t - 15)(t - 20) \\&= -4.2541 + 21.265t + 0.13204t^2 + 0.005434t^3, \quad 10 \leq t \leq 22.5\end{aligned}$$

Note that the polynomial is valid between $t = 10$ and $t = 22.5$ and hence includes the limits of $t = 11$ and $t = 16$. So

$$\begin{aligned}
& s(16) - s(11) \\
&= \int_{11}^{16} v(t) dt \\
&= \int_{11}^{16} (-4.2541 + 21.265t + 0.13204t^2 + 0.0054347t^3) dt \\
&= \left[-4.2541t + 21.265\frac{t^2}{2} + 0.13204\frac{t^3}{3} + 0.0054347\frac{t^4}{4} \right]_{11}^{16} \\
&= \left[-4.2541(16) + 21.265\frac{(16)^2}{2} + 0.13204\frac{(16)^3}{3} + 0.0054347\frac{(16)^4}{4} \right] \\
&\quad - \left[-4.2541(11) + 21.265\frac{(11)^2}{2} + 0.13204\frac{(11)^3}{3} + 0.0054347\frac{(11)^4}{4} \right] \\
&= 1605m
\end{aligned}$$

(c). The acceleration at $t = 16$ is given by

$$a(16) = \frac{d}{dt}v(t)|_{t=16}$$

$$a(t) = \frac{d}{dt}v(t)$$

$$= \frac{d}{dt}(-4.2541 + 21.265t + 0.13204t^2 + 0.0054347t^3)$$

$$= (0) + 21.265(1) + 0.13204(2 \times t^{(2-1)}) + 0.0054347(3 \times t^{(3-1)})$$

$$= 21.265 + 0.26408t + 0.016304t^2$$

$$a(16) = 21.265 + 0.26408(16) + 0.016304(16)^2$$

$$= 29.664m/s^2$$

x	0	1	2	3	4
$y = f(x)$	2	3	6	11	18

Interpolation: Finding the value of $f(x)$ at some value of $x = 1.4$ in between two tabular values, e.g., between $f(x) = 3$ and $f(x) = 6$.

Inverse interpolation: If a value of $f(x)$ between $f(x) = 6$ and $f(x) = 11$ is known, inverse interpolation is to find the corresponding value of x .

Extrapolation: Determining the value of $f(x)$ at point $x = 5$ (outside the range of tabular values) .